how do I prove that eval is transitive?

hw8/prob02.lean
@@ -1,17 +1,60 @@
 -- IMPORTANT: See `src/lnat.lean` for the formalization of Lnat.
 import .src.lnat
 
+-- Condition 1: There exists an expression e2 such that e1 → e2.
+-- Condition 2: The proof of e1 → e2 uses all the three inference rules for e → e′.
+
+-- Rules:
+-- 1. E-Left:          e1 → e1' -> e1 ⊛ e2 → e1' ⊛ e2
+-- 2. E-Right: e1 val, e2 → e2' -> e1 ⊛ e2 → e1 ⊛ e2'
+-- 3. E-Op:                        n1 ⊛ n2 → n1 * n2
+
+-- e1: (1*2) + (4/2)
+-- e2: 4
+
+--    (1*2) + (4/2)
+-- ->   2   + (4/2) E-Left
+-- ->   2   +   2   E-Right
+-- ->       4       E-Op
+
+def e1left : Expr := Expr.Op Op.Mul (Expr.Num 1) (Expr.Num 2)
+def e1right : Expr := Expr.Num 3
+
 def e1 : Expr :=
-  -- FILL IN HERE.
-  sorry
+  Expr.Op Op.Add
+  -- (Expr.Num 2)
+  e1left
+  e1right
+  -- (Expr.Op Op.Div (Expr.Num 4) (Expr.Num 2))
+
+def e1b : Expr :=
+  Expr.Op Op.Add
+  (Expr.Num 2)
+  (Expr.Num 3)
 
 def e2 : Expr :=
-  -- FILL IN HERE.
+  Expr.Num 5
+
+lemma eval_e1be2 :
+  e1b ↦ e2 :=
+  eval.EOp Op.Add 2 3
+
+-- e ↦ e' := eval e e'
+lemma eval_e1e1b :
+  e1 ↦ e1b :=
+  eval.ELeft Op.Add e1left (Expr.Num 2) e1right (eval.EOp Op.Mul 1 2)
+
+lemma eval_trans {a b c : Expr}
+  (e1: a↦b) (e2: b↦c) : a ↦ c :=
   sorry
 
-lemma eval_example :
+theorem eval_full :
   e1 ↦ e2 :=
-begin
-  -- FILL IN HERE.
-  sorry
-end
+  eval_trans eval_e1e1b eval_e1be2
+  -- eval.ELeft Op.Add e1left (Expr.Num 2) e1right (eval.EOp Op.Mul 1 2)
+  -- eval (Expr.Op Op.Add e1left e1right) (Expr.Num 5)
+
+-- begin
+--   apply eval.ELeft Op.Add,
+--   apply eval.EOp,
+-- end
